src/QUIC.Parse.fsti
@@ -43,9 +43,9 @@ val format_header_is_retry: h: header -> Lemma
 
 val format_header_pn_length: h: header -> Lemma
   (requires (~ (is_retry h)))
-  (ensures (BF.get_bitfield (U8.v (S.index (format_header h) 0)) 0 2 == U32.v (pn_length h)))
+  (ensures (BF.get_bitfield (U8.v (S.index (format_header h) 0)) 0 2 == U32.v (pn_length h) - 1))
 
-val pn_offset: (h: header { ~ (is_retry h) }) -> GTot (n: nat { 0 < n /\ n + U32.v (pn_length h) <= header_len h })
+val pn_offset: (h: header { ~ (is_retry h) }) -> GTot (n: nat { 0 < n /\ n + U32.v (pn_length h) == header_len h }) // need to know that packet number is the last field of the format
 
 val putative_pn_offset: (cid_len: nat) -> (x: bytes) -> GTot (option (y: nat {0 < y /\ y <= Seq.length x}))
 
